code/ecdsa/Hacl.Impl.EC.LowLevel.fsti
@@ -142,7 +142,7 @@ val felem_add: #c: curve -> a: felem c -> b: felem c -> out: felem c ->
       as_nat c h1 out == (as_nat c h0 a + as_nat c h0 b) % getPrime c /\
       as_nat c h1 out == toDomain #c ((fromDomain #c (as_nat c h0 a) + fromDomain #c (as_nat c h0 b)) % getPrime c)))
 
-[@CInline]
+inline_for_extraction noextract
 val felem_double: #c: curve -> a: felem c -> out: felem c ->
   Stack unit
     (requires (fun h0 ->
@@ -152,7 +152,7 @@ val felem_double: #c: curve -> a: felem c -> out: felem c ->
       as_nat c h1 out == (2 * as_nat c h0 a) % getPrime c /\
       as_nat c h1 out == toDomain #c (2 * fromDomain #c (as_nat c h0 a) % getPrime c)))
 
-[@CInline]
+inline_for_extraction noextract
 val felem_sub: #c: curve -> a: felem c -> b: felem c -> out: felem c ->
   Stack unit
   (requires (fun h0 ->
